Pauline/Dynamics.lean
@@ -8,18 +8,69 @@ namespace Pauline
 def isVal : Exp → Bool
 | .scon _
 | .lam _ _
-| .tuple [] => true
+| .extern _ _
+| .tuple []        => true
 | .tuple (e :: es) => isVal e ∧ isVal (.tuple es)
 | .typed _ _
+| .var _
 | .case _ _
 | .ite _ _ _
 | .app _ _
 | .let_in _ _
-| .var _
 | .raise _ => false
+
+def Exn.bind   : Exp  := .var "Bind"
+def Exn.match  : Exp  := .var "Match"
+def Exn.div    : Exp  := .var "Div"
+
+def Extern.add : Exp :=
+  .extern "+" (fun | [.int x, .int y] => .scon (.int (x + y))
+                   | _ => panic! "Extern TC Failure" )
+def Extern.sub : Exp :=
+  .extern "-" (fun | [.int x, .int y] => .scon (.int (x - y))
+                   | _ => panic! "Extern TC Failure" )
+def Extern.mul : Exp :=
+  .extern "*" (fun | [.int x, .int y] => .scon (.int (x * y))
+                   | _ => panic! "Extern TC Failure" )
+def Extern.div : Exp :=
+  .extern "div" (fun | [.int x, .int y] => .scon (.int (x / y))
+                     | _ => panic! "Extern TC Failure" )
+def Extern.eq : Exp :=
+  .extern "=" (fun | [.int x, .int y] => .scon (.bool (x = y))
+                   | _ => panic! "Extern TC Failure" )
+def Extern.neq : Exp :=
+  .extern "<>" (fun | [.int x, .int y] => .scon (.bool (x ≠ y))
+                    | _ => panic! "Extern TC Failure" )
+def Extern.lt : Exp :=
+  .extern "<" (fun | [.int x, .int y] => .scon (.bool (x < y))
+                   | _ => panic! "Extern TC Failure" )
+def Extern.gt : Exp :=
+  .extern ">" (fun | [.int x, .int y] => .scon (.bool (x > y))
+                   | _ => panic! "Extern TC Failure" )
+def Extern.le : Exp :=
+  .extern "<=" (fun | [.int x, .int y] => .scon (.bool (x ≤ y))
+                    | _ => panic! "Extern TC Failure" )
+def Extern.ge : Exp :=
+  .extern "<=" (fun | [.int x, .int y] => .scon (.bool (x ≥ y))
+                    | _ => panic! "Extern TC Failure" )
 
 structure State where
   values : HashMap Ident { e // isVal e }
+
+instance : Inhabited State where
+  default :=
+    ⟨ HashMap.empty
+      |>.insert "+"   ⟨Extern.add, by decide⟩
+      |>.insert "-"   ⟨Extern.sub, by decide⟩
+      |>.insert "*"   ⟨Extern.mul, by decide⟩
+      |>.insert "div" ⟨Extern.div, by decide⟩
+      |>.insert "="   ⟨Extern.eq , by decide⟩
+      |>.insert "<>"  ⟨Extern.neq, by decide⟩
+      |>.insert "<"   ⟨Extern.lt , by decide⟩
+      |>.insert ">"   ⟨Extern.gt , by decide⟩
+      |>.insert "<="  ⟨Extern.le , by decide⟩
+      |>.insert ">="  ⟨Extern.ge , by decide⟩
+    ⟩
 
 def Pat.bindsIdent (i : Ident) : Pat → Bool
 | wild            => false
@@ -43,6 +94,7 @@ def subst : Exp → Exp
 | .let_in _ _ => panic! "unimplemented"
 | .var i => if x = i then e else .var i
 | .raise e' => .raise (subst e')
+| .extern name f => .extern name f
 
 def substList : List Exp → List Exp
 | [] => []
@@ -53,22 +105,64 @@ def substMatches : List (Pat × Exp) → List (Pat × Exp)
 | (p,e')::ms => (if p.bindsIdent x then (p,e') else (p, subst e')) :: substMatches ms
 end
 
+partial def substPat (body : Exp) : { e // isVal e } → Pat → Exp
+  | _, .wild => body
+  | ⟨.typed e _, _⟩, p => substPat body ⟨e, sorry⟩ p
+  | e, .typed p _ => substPat body e p
+  | e, .bind name => subst e.val name body
+  | ⟨.scon e_sc, _⟩, .scon p_sc =>
+    if e_sc = p_sc then body else .raise Exn.bind
+  | ⟨.tuple [], _⟩, .tuple [] => body
+  | ⟨.tuple (e::es), _⟩, .tuple (p::ps) =>
+    let res := substPat body ⟨e, sorry⟩ p
+    match substPat body ⟨.tuple es, sorry⟩ (.tuple ps) with
+    | .tuple res_rest => .tuple (res :: res_rest)
+    | _ => .raise Exn.bind
+  | _, .tuple _ => .raise Exn.bind
+  | e, .layer name _ p => substPat (subst e.val name body) e p
+  | _, _ => .raise Exn.bind
+
+def callExtern (f : List SCon → Exp) : { e // isVal e } → Exp
+  | ⟨.scon sc, _⟩ => f [sc]
+  | ⟨.tuple [], _⟩ => f []
+  | ⟨.tuple es, _⟩ => f (extractSCon es)
+  | _ => panic! s!"Invalid extern call"
+where extractSCon : List Exp → List SCon
+  | [] => []
+  | (.scon sc) :: es => sc :: extractSCon es
+  | (.tuple vs) :: es => extractSCon vs ++ extractSCon es
+  | _ => []
+
 inductive StepExp : State × Exp → State × Exp → Prop
 | tupleNilStep
   : StepExp (s, .tuple []) (s, .tuple [])
-| tupleConsStep {e es}
-  (h_e : StepExp (s,e) (s',e')) (h_es : StepExp (s', .tuple es) (s'', .tuple es'))
-  : StepExp (s, .tuple (e :: es)) (s'', .tuple (e' :: es'))
+| tupleHdStep (he : StepExp (s, e) (s', e'))
+  : StepExp (s, .tuple (e::es)) (s', .tuple (e'::es))
+| tupleTlStep (he : isVal e) (hes : StepExp (s, .tuple es) (s', .tuple es'))
+  : StepExp (s, .tuple (e::es)) (s', .tuple (e::es'))
+-- | tupleConsStep {e es}
+  -- (h_e : StepExp (s,e) (s',e')) (h_es : StepExp (s', .tuple es) (s'', .tuple es'))
+  -- : StepExp (s, .tuple (e :: es)) (s'', .tuple (e' :: es'))
 | typedStep
   : StepExp (s, .typed e t) (s, e)
 | varStep (h : s.values.find? i = some e)
-  : StepExp (s, .var i) (s, e)
+  : StepExp (s, .var i) (s, e.val)
 | appStepL (hf : StepExp (s, f) (s', f'))
   : StepExp (s, .app f e) (s', .app f' e)
 | appStepR (hf : isVal f) (he : StepExp (s, e) (s', e'))
   : StepExp (s, .app f e) (s', .app f e')
-| appStep (he : isVal e) (he' : e' = sorry)
+| appStep (he : isVal e) (he' : e' = substPat body ⟨e, he⟩ p)
   : StepExp (s, .app (.lam p body) e) (s, e')
+| raiseStep (he : StepExp (s, e) (s', e'))
+  : StepExp (s, .raise e) (s', .raise e')
+| externStep (he : isVal e) (he' : e' = callExtern f ⟨e, he⟩)
+  : StepExp (s, .app (.extern name f) e) (s, e')
+| iteStepB {b b' t f : Exp} (hb : StepExp (s, b) (s', b'))
+  : StepExp (s, .ite b t f) (s', .ite b' t f)
+| iteStepT (hb : b = .scon (.bool true))
+  : StepExp (s, .ite b t f) (s, t)
+| iteStepF (hb : b = .scon (.bool false))
+  : StepExp (s, .ite b t f) (s, f)
 
 def StepsNExp : Nat → State × Exp → State × Exp → Prop
 | 0 => λ (s, e) (s'', e'') => s = s'' ∧ e = e''
@@ -88,7 +182,7 @@ theorem StepsExp.trans (h1 : StepsExp x y) (h2 : StepsExp y z)
   clear h1 h2
   refine ⟨n1+n2, ?_⟩
   match n2 with
-  | 0 => 
+  | 0 =>
     simp [StepsNExp] at h2' ⊢
     match h2' with
     | ⟨rfl, rfl⟩ =>
@@ -120,3 +214,98 @@ instance : Trans StepsExp StepExp StepsExp where
 
 instance : Trans StepsExp StepsExp StepsExp where
   trans h1 h2 := h1.trans h2
+
+inductive StepRes (init : State × Exp)
+  | val   : isVal init.2 → StepRes init
+  | var   : Ident → StepRes init -- free variable
+  | raise : Ident → StepRes init
+  | step  : (s : State) → (e : Exp) → StepExp init (s, e) → StepRes init
+
+def StepRes.toString : StepRes init → String
+  | .val _ => "val"
+  | .var x => s!"free-var: {x}"
+  | .raise x => s!"raise {x}"
+  | .step _s' e' _h => s!"stepped: {e'}"
+instance : ToString (StepRes init) := ⟨StepRes.toString⟩
+
+def step (s : State) (exp : Exp) : StepRes (s, exp) :=
+  match hexp : exp with
+  | .scon sc  => .val (by simp [isVal])
+  | .var x    =>
+    match h : s.values.find? x with
+    | some e => .step s e.val (.varStep h)
+    | none   => .var x
+  | .tuple [] => .val (by simp [isVal])
+  | .tuple (e :: es) =>
+    match step s e with
+    | .val he =>
+      match step s (.tuple es) with
+      | .val hes => .val (by simp [isVal]; exact ⟨he, hes⟩)
+      | .var x => .var x
+      | .raise exn => .raise exn
+      | .step s' (.tuple es') hes =>
+        .step s' (.tuple (e::es')) (.tupleTlStep he hes)
+    | .var x => .var x
+    | .raise exn => .raise exn
+    | .step s' e' he => .step s' (.tuple (e'::es)) (.tupleHdStep he)
+  | .raise e =>
+    match step s e with
+    | .var x => .var x
+    | .raise exn => .raise exn
+    | .step s' e' h => .step s' (.raise e') (.raiseStep h)
+    | _ => .raise "INVALID"
+  | .let_in _ _ => .raise "FAIL: Implement"
+  | .app f e =>
+    match step s f with
+    | .step s' f' h => .step s' (.app f' e) (.appStepL h)
+    | .raise exn    => .raise exn
+    | .var x        => .var x
+    | .val hf        =>
+      match step s e with
+      | .step s' e' he => .step s' (.app f e') (.appStepR hf he)
+      | .raise exn     => .raise exn
+      | .var x         => .var x
+      | .val he =>
+          match f with
+          | .lam p body =>
+            .step s (substPat body ⟨e, he⟩ p) (.appStep he rfl)
+          | .extern _ exe =>
+            .step s (callExtern exe ⟨e, he⟩) (.externStep he rfl)
+          | _ => .raise s!"FAIL: SOMETHING WENT WRONG {Exp.app f e}"
+  | .typed e τ => .step s e .typedStep
+  | .ite b t f =>
+    match b with
+    | .scon (.bool true)  => .step s t (.iteStepT rfl)
+    | .scon (.bool false) => .step s f (.iteStepF rfl)
+    | _ =>
+      match step s b with
+      | .step s' b' h => .step s' (.ite b' t f) (.iteStepB sorry)
+      | .var x => .var x
+      | .raise exn => .raise exn
+      | _ => .raise s!"FAIL: SOMETHING WENT WRONG ITE {b}"
+  | .case e cl => .raise "FAIL: Implement"
+  | .lam p body => .val (by simp [isVal])
+  | .extern _ exe => .val (by simp [isVal])
+
+inductive EvalRes (init : State × Exp)
+| val : (e : {e // isVal e}) → StepsExp init (s, e.val) → EvalRes init
+| var : Ident → StepsExp init (s, e) → EvalRes init
+| raise : Ident → EvalRes init
+deriving Inhabited
+
+def EvalRes.toString : EvalRes init → String
+  | .val e _ => s!"val {e.val}"
+  | .var (e:=e) x _ => s!"free-var: {x} in {e}"
+  | .raise x => s!"raise {x}"
+instance : ToString (EvalRes init) := ⟨EvalRes.toString⟩
+
+partial def eval_acc (s : State) (e : Exp) (acc : StepsExp init (s, e))
+    : EvalRes init  :=
+  match step s e with
+  | .step s' e' h => eval_acc s' e' (trans acc h)
+  | .val h => .val ⟨e, h⟩ acc
+  | .var x => .var x acc
+  | .raise exn => .raise exn
+
+def eval (s : State) (e : Exp) : EvalRes (s, e) :=
+  eval_acc s e (⟨0, by simp [StepsNExp]⟩)
