Pauline/Syntax.lean
@@ -5,15 +5,16 @@ open Std
 namespace Pauline
 
 def Ident := String
-deriving DecidableEq, Hashable, Repr
+deriving DecidableEq, Hashable, Repr, ToString, Inhabited
 
 inductive SCon
 | int (n : Int)
+| bool (b : Bool) -- temp
 | str (s : String)
-deriving Repr
+deriving Repr, DecidableEq
 
 inductive Typ
-| int | string
+| int | string | bool
 | exn
 | prod (ts : List Typ)
 | arr (dom cod : Typ)
@@ -44,18 +45,17 @@ inductive Exp
 | ite (b : Exp) (t : Exp) (f : Exp)
 | case (e : Exp) (clauses : List (Pat × Exp))
 | lam (p : Pat) (body : Exp)
-deriving Repr, Inhabited
+| extern (name : String) (exe : List SCon → Exp) -- a built in function/op
+deriving Inhabited
 
 inductive Dec
 | val (p : Pat) (exp : Exp)
 | valrec (p : Pat) (expPat : Pat) (expBody : Exp)
 | «fun» (name : Ident) (pats : List.Nonempty Pat) (ret : Option Typ) (body : Exp)
-deriving Repr
 end
 
 structure Prog where
   decls : List Dec
-deriving Repr
 
 
 instance : OfNat Exp n where
@@ -63,3 +63,71 @@ instance : OfNat Exp n where
 
 instance : Coe Nat Exp where
   coe n := .scon (.int n)
+
+def SCon.toString : SCon → String
+  | .int n => s!"{n}"
+  | .bool b => s!"{b}"
+  | .str s => s!"\"{s}\""
+instance : ToString SCon := ⟨SCon.toString⟩
+instance : Repr SCon := ⟨(fun scon _ => scon.toString)⟩
+
+partial def Typ.toString : Typ → String
+  | .int        => "int"
+  | .bool       => "bool"
+  | .string     => "string"
+  | .exn        => "exn"
+  | .prod ts    => s!"({", ".intercalate (ts.map toString)})"
+  | .arr fn arg => s!"{toString fn} -> {toString arg}"
+  | .tyvar id   => s!"'{id}"
+  | .tycon name args => s!"({", ".intercalate (args.map toString)}) {name}"
+instance : ToString Typ := ⟨Typ.toString⟩
+instance : ToString (Option Typ) where
+  toString | none   => ""
+           | some τ => s!": {τ}"
+instance : Repr Typ := ⟨(fun τ _ => τ.toString)⟩
+
+partial def Pat.toString : Pat → String
+  | .wild      => "_"
+  | .bind name => name
+  | .scon sc   => SCon.toString sc
+  | .tuple ps  => s!"({", ".intercalate (ps.map toString)})"
+  | .typed p τ => s!"{toString p} : {τ}"
+  | .layer name .none p     => s!"{name} as {toString p}"
+  | .layer name (.some τ) p => s!"({name} : {τ}) as {toString p}"
+instance : ToString Pat := ⟨Pat.toString⟩
+instance : ToString (List Pat) :=
+  ⟨fun ps => s!"({", ".intercalate (ps.map toString)})"⟩
+instance : Repr Pat := ⟨(fun p _ => p.toString)⟩
+
+mutual
+partial def Exp.toString : Exp → String
+  | .scon sc    => s!"({sc})"
+  | .var name   => name
+  | .tuple es   => s!"({", ".intercalate (es.map Exp.toString)})"
+  | .raise e    => s!"raise {e.toString}"
+  | .let_in d e => s!"let {d.toString} in {e.toString}"
+  | .app fn arg => s!"{fn.toString} {arg.toString}"
+  | .typed e τ  => s!"{e.toString} : {τ}"
+  | .ite b t f  => s!"if {b.toString} then {t.toString} else {f.toString}"
+  | .case e cl  =>
+    let cl_str :=
+      " | ".intercalate (cl.map (fun (p, e) => s!"{p} => {e.toString}"))
+    s!"case {e.toString} of {cl_str}"
+  | .lam p body => s!"fn {p} => {body.toString}"
+  | .extern f _ => s!"fn ? => extern_{f}"
+
+partial def Dec.toString : Dec → String
+  | .val p e => s!"val {p} = {e.toString}"
+  | .valrec p ep body => s!"val rec {p} = fn {ep} => {body.toString}"
+  | .fun name ps ret? body =>
+    s!"fun {name} {ps.val} {ret?} = {body.toString}"
+end
+instance : ToString Exp := ⟨Exp.toString⟩
+instance : ToString Dec := ⟨Dec.toString⟩
+instance : Repr Exp     := ⟨(fun e _ => e.toString)⟩
+instance : Repr Dec     := ⟨(fun d _ => d.toString)⟩
+
+def Prog.toString : Prog → String
+  | ⟨decls⟩ => "\n\n".intercalate (decls.map Dec.toString)
+instance : ToString Prog := ⟨Prog.toString⟩
+instance : Repr Prog     := ⟨(fun p _ => p.toString)⟩
